lakefile.lean
@@ -1,0 +1,7 @@
+import Lake
+open Lake DSL
+
+package «nesylink» where
+
+lean_lib LogicSubmissions where
+  srcDir := "."
